Proved merge sort's correctness

MergeSort.v
@@ -1,4 +1,5 @@
 Require Import Arith Div2 List Orders Sorted Permutation Program.
+Require Omega.
 
 Module MergeSort (Import X : TotalTransitiveLeBool').
   Local Coercion is_true : bool >-> Sortclass.
@@ -13,36 +14,37 @@ Module MergeSort (Import X : TotalTransitiveLeBool').
       match xs as xs0 return
         StronglySorted leb xs0 ->
         forall ys, StronglySorted leb ys ->
-        { zs | StronglySorted leb zs /\ Permutation zs (xs0 ++ ys) } with
+        { zs | StronglySorted leb zs
+            /\ Permutation zs (xs0 ++ ys) } with
       | [] => fun _ ys _ => exist _ ys _
       | x :: xs' => fun _ =>
           fix merge' ys :=
             match ys with
             | [] => fun _ => exist _ (x :: xs') _
             | y :: ys' => fun _ => 
-                match (x <=? y) as b return
+                (if x <=? y as b return
                   x <=? y = b ->
-                  { zs | StronglySorted leb zs /\ Permutation zs (x :: xs' ++ y :: ys') }
-                with
-                | true => fun _ =>
-                    let (zs, _) := merge xs' _ (y :: ys') _ in
-                    exist _ (x :: zs) _
-                | false => fun _ =>
-                    let (zs, _) := merge' ys' _ in
-                    exist _ (y :: zs) _
-                end eq_refl
+                  { zs | StronglySorted leb zs
+                      /\ Permutation zs (x :: xs' ++ y :: ys') }
+                then fun _ =>
+                  let (zs, _) := merge xs' _ (y :: ys') _ in
+                  exist _ (x :: zs) _
+                else fun _ =>
+                  let (zs, _) := merge' ys' _ in
+                  exist _ (y :: zs) _) eq_refl
             end
       end);
       simpl in *;
       try clear merge';
       repeat rewrite app_nil_r in *;
-      repeat split;
-      repeat apply SSorted_cons;
       repeat match goal with
       | H : StronglySorted _ (_ :: _) |- _ =>
           inversion H; clear H; subst
       | H : _ /\ _ |- _ => destruct H
-      end; eauto;
+      end;
+      repeat split;
+      repeat apply SSorted_cons;
+      eauto;
       repeat match goal with
       | H : Forall ?P ?l |- _ =>
           assert (forall x, In x l -> P x)
@@ -65,7 +67,7 @@ Module MergeSort (Import X : TotalTransitiveLeBool').
     - apply Permutation_cons_app with (l1 := x :: xs').
       eauto.
   Defined.
-      
+
   Definition meld : forall xss,
     Forall (StronglySorted leb) xss ->
     { xss' | length xss' = div2 (S (length xss))
@@ -83,13 +85,93 @@ Module MergeSort (Import X : TotalTransitiveLeBool').
       end);
       simpl in *; clear meld;
       repeat rewrite app_nil_r in *;
-      repeat split; eauto;
       repeat match goal with
       | H : Forall _ (_ :: _) |- _ =>
           inversion H; clear H; subst
       | H : _ /\ _ |- _ => destruct H
-      end; eauto.
+      end;
+      repeat split; eauto.
     rewrite app_assoc.
     apply Permutation_app; eauto.
   Defined.
+
+  Definition merge_sort xs :
+    { xs' | StronglySorted leb xs' /\ Permutation xs' xs }.
+  Proof.
+    refine (let (xs', _) := Fix
+        (well_founded_ltof _ (@length _))
+        (fun xss =>
+          Forall (StronglySorted leb) xss ->
+          Permutation (fold_right (@app _) [] xss) xs ->
+          { xs' | StronglySorted leb xs' /\ Permutation xs' xs })
+        (fun xss =>
+          match xss with
+          | [] => fun _ _ _ => exist _ [] _
+          | [xs] => fun _ _ _ => exist _ xs _
+          | xs :: ys :: xss => fun iter_meld _ _ =>
+              let (xss', _) := meld (xs :: ys :: xss) _ in
+              iter_meld xss' _ _ _
+          end)
+        (map (fun x => [x]) xs) _ _ in
+      exist _ xs' _);
+      simpl in *;
+      repeat rewrite app_nil_r in *;
+      repeat match goal with
+      | H : Forall _ (_ :: _) |- _ =>
+          inversion H; clear H; subst
+      | H : _ /\ _ |- _ => destruct H
+      end;
+      repeat split;
+      eauto.
+    - unfold ltof.
+      simpl in *.
+      destruct (length xss0).
+      + omega.
+      + rewrite H.
+        apply le_n_S.
+        apply lt_div2 with (n := S (S n)).
+        omega.
+    - apply Forall_forall.
+      intros ? HIn.
+      apply in_map_iff in HIn.
+      destruct HIn as [? []].
+      subst.
+      eauto.
+    - induction xs; simpl; eauto.
+  Defined.
 End MergeSort.
+
+Module Nat_as_TTLB <: TotalTransitiveLeBool.
+  Let t := nat.
+
+  Definition leb m n :=
+    if le_dec m n then true
+    else false.
+
+  Definition leb_total m n :
+    leb m n = true \/ leb n m = true.
+  Proof.
+    unfold leb.
+    destruct (le_dec m n);
+      destruct (le_dec n m);
+        solve [ eauto | omega ].
+  Qed.
+
+  Definition leb_trans l m n :
+    leb l m = true ->
+    leb m n = true ->
+    leb l n = true.
+  Proof.
+    unfold leb.
+    intros.
+    destruct (le_dec l m);
+      destruct (le_dec m n);
+        destruct (le_dec l n);
+          solve [ congruence | omega ].
+  Qed.
+End Nat_as_TTLB.
+
+Module NatSort := MergeSort Nat_as_TTLB.
+
+(* FUCKIN' HEAVY COMPUTATION *)
+(* Eval compute in NatSort.merge_sort [1; 1; 4; 5; 1; 4]. *)
